Reduce to zero

Hoare2.v
@@ -1,3 +1,36 @@
 Require Export Hoare.
 
+Definition reduce_to_zero' : com :=
+    WHILE BNot (BEq (AId X) (ANum 0)) DO
+        X ::= AMinus (AId X) (ANum 1)
+    END.
+
+Theorem reduce_to_zero_correct' :
+    {{ fun st => True }}
+    reduce_to_zero'
+    {{ fun st => st X = 0 }}.
+Proof.
+    unfold reduce_to_zero'.
+    (* transform the post-condition; then hoare_while *)
+    eapply hoare_consequence_post.
+    Case "Hoare_while".
+        apply hoare_while.
+        (* transform pre-condition; then hoare_assg *)
+        eapply hoare_consequence_pre.
+        SCase "assignment".
+            apply hoare_asgn.
+        SCase "pre-condition weakening".
+            intros st [HT GuardTrue]. unfold assn_sub. apply HT.
+    Case "strenghening the post-condition".
+        intros st [HT GuardFalse].
+        unfold bassn in GuardFalse. simpl in GuardFalse.
+        SearchAbout [not true].
+        rewrite -> not_true_iff_false in GuardFalse.
+        SearchAbout [negb false].
+        rewrite negb_false_iff in GuardFalse.
+        SearchAbout [beq_nat true].
+        apply beq_nat_true in GuardFalse.
+        apply GuardFalse.
+Qed.
+
 
